Progress on SMTLIB generator.

lean/deps/galois_stdlib/src/galois/data/buffer.lean
@@ -4,9 +4,43 @@ Provides a decidable_eq instance for buffer.
 import data.buffer.basic -- from mathlib
 
 import galois.data.array
+import galois.data.char
+import galois.data.nat
 
 namespace buffer
 
+@[simp]
+theorem size_append_array {α} {n : nat} (nz : n > 0)  (x : buffer α) (y : array n α) (j : nat) (j_lt : j < n)
+: buffer.size (buffer.append_array nz x y j j_lt) = x.size + j + 1 :=
+begin
+  revert x,
+  induction j,
+  case nat.zero {
+    intro x,
+    cases x,
+    simp [append_array, size],
+  },
+  case nat.succ : j ind {
+    intro x,
+    cases x with m b,
+    simp [append_array, ind],
+    simp [size, nat.succ_add, nat.add_succ],
+  },
+end
+
+@[simp]
+theorem size_append {α} (x y : buffer α)
+: (x ++ y).size = x.size + y.size :=
+begin
+  cases y with n b,
+  cases n,
+  case nat.zero { simp [size, append, buffer.append], },
+  case nat.succ : n {
+    simp [size, append, buffer.append, size_append_array, nat.succ_add],
+  }
+end
+
+@[simp]
 theorem to_list_length {α} (b: buffer α)
 : list.length (buffer.to_list b) = b.size :=
 begin
@@ -24,7 +58,6 @@ begin
   cases b with n a,
   simp only [read, to_list, array.to_list_nth_le', to_array],
 end
-
 
 /-- Empty buffer converted to array is same as array.nil -/
 @[simp]
@@ -48,4 +81,199 @@ end
 theorem to_char_buffer_as_string (l:list char)
 : l.as_string.to_char_buffer = l.to_buffer := eq.refl l.to_buffer
 
+@[simp]
+theorem size_push_back {α} (b:buffer α) (c:α)
+: (buffer.push_back b c).size = b.size + 1 :=
+begin
+  cases b,
+  trivial,
+end
+
+@[simp]
+theorem size_append_list {α} (b:buffer α) (l:list α)
+: (buffer.append_list b l).size = l.length + b.size :=
+begin
+  revert b,
+  induction l,
+  case list.nil {
+    intro b,
+    simp [buffer.append_list, nat.zero_add],
+  },
+  case list.cons : x r ind {
+    intro b,
+    simp only [buffer.append_list, ind, size_push_back, list.length_cons,
+               nat.add_succ, nat.add_zero, nat.succ_add],
+  },
+end
+
+/- Prove definition of reading from concatenation of two buffers. -/
+theorem read_append_array {α} {n:ℕ} (nz : n > 0) (x : buffer α) (b : array n α) (j:ℕ) (j_lt : j < n)
+   (i : fin (append_array nz x b j j_lt).size)
+: read (append_array nz x b j j_lt) i =
+  if h : i.val < x.size then
+    x.read ⟨i.val, h⟩
+  else
+    let q : n + (i.val - x.size) - (j + 1)  < n :=
+      begin
+        cases i with i i_lt,
+        let nz_lt : 0 < n := nz,
+        simp only [nat.sub_lt_to_add, nz_lt, or_true, and_true],
+        apply nat.add_lt_add_left,
+        have x_le := le_of_not_lt h,
+        simp [nat.sub_lt_to_add, x_le],
+        simp [size_append_array] at i_lt,
+        exact i_lt,
+      end in
+    array.read b ⟨n + (i.val - x.size) - (j + 1), q⟩ :=
+begin
+  revert x,
+  induction j,
+  case nat.zero {
+    intros x i,
+    cases i with i i_lt,
+    cases x with m a,
+    dsimp [append_array, read, size],
+    simp [array.read_push_back_lt_iff],
+    cases (decide (i < m)),
+    case decidable.is_true : lt {
+      simp [lt],
+    },
+    case decidable.is_false : not_lt {
+      simp [not_lt],
+      dsimp [append_array, size] at i_lt,
+      have p : i ≤ m := nat.le_of_lt_succ i_lt,
+      have q : i-m=0 := nat.sub_eq_zero_of_le p,
+      simp [q],
+    },
+  },
+  case nat.succ : j ind {
+    intros x i,
+    cases i with i i_outer_lt,
+    cases x with m a,
+    dsimp [append_array, size],
+    simp [ind],
+    dsimp [size],
+    cases nat.lt_trichotomy i m,
+    case or.inl : i_lt {
+      have i_lt_m_p_1 : i < m + 1 := nat.lt_succ_of_lt i_lt,
+      simp [i_lt, i_lt_m_p_1, read, array.read_push_back_lt_iff],
+    },
+    case or.inr : i_geq {
+      cases i_geq,
+      case or.inl : i_eq {
+        have i_lt_m_p_1 : i < m + 1, { simp [i_eq, nat.zero_lt_succ], },
+        simp [i_lt_m_p_1, i_eq, read, array.read_push_back_lt_iff],
+        apply (congr_arg (array.read b)),
+        apply fin.eq_of_veq,
+        simp [nat.succ_add, nat.add_succ, nat.sub_sub],
+      },
+      case or.inr : i_gt {
+        have not_i_lt_m : ¬ (i < m) := not_lt_of_lt i_gt,
+        have not_i_lt_m_p_1 : ¬ (i < m + 1), {
+          apply not_lt_of_le,
+          exact i_gt,
+        },
+        simp [not_i_lt_m, not_i_lt_m_p_1],
+        apply (congr_arg (array.read b)),
+        apply fin.eq_of_veq,
+        have not_i_m_zero : ¬(i - m = 0), {
+          intro eq_zero,
+          have not_i_gt := not_lt_of_ge (nat.le_of_sub_eq_zero eq_zero),
+          exact (not_i_gt i_gt),
+        },
+        simp [fin.val, nat.succ_add, nat.add_succ, nat.sub_succ
+             , nat.add_pred, nat.pred_sub, not_i_m_zero],
+      },
+    },
+  },
+end
+
+/-- Proof needed for starting theorem about read of append. -/
+theorem read_append.pr1 {α} (x y : buffer α) (i : fin ((x++y).size)) (h : ¬(i.val < x.size ))
+: i.val - buffer.size x < buffer.size y :=
+begin
+  have q : buffer.size x ≤ i.val := le_of_not_lt h,
+  simp [nat.sub_lt_left_iff_lt_add q],
+  exact trans_rel_left _ i.is_lt (size_append _ _),
+end
+
+/- Prove definition of reading from concatenation of two buffers. -/
+theorem read_append {α} (x y : buffer α) (i : fin ((x++y).size))
+: (x ++ y).read i =
+  if h : i.val < x.size then
+    x.read ⟨i.val, h⟩
+  else
+    y.read ⟨i.val - x.size, read_append.pr1 x y i h⟩ :=
+begin
+  cases y with n b,
+  cases n,
+  case nat.zero {
+    cases i with i i_lt,
+    dsimp [has_append.append, buffer.append] at i_lt,
+    -- Simplify left-hand side
+    dsimp [has_append.append, buffer.append],
+    -- Simplify right-hand side
+    simp [i_lt],
+  },
+  case nat.succ : n {
+    cases i with i i_lt,
+    dsimp [has_append.append, buffer.append],
+    simp [read_append_array ],
+    dsimp [fin.val],
+    cases decide (i < size x),
+    case decidable.is_true : i_lt { simp [i_lt], },
+    case decidable.is_false : not_i_lt {
+      simp [not_i_lt, read],
+      apply congr_arg (array.read b),
+      exact fin.eq_of_veq (eq.refl _),
+    },
+  },
+end
+
+protected
+def le {α} [h:linear_order α] : buffer α → buffer α → Prop
+| ⟨m,a⟩ ⟨n,b⟩ := array.lex_le a b
+
+instance {α} [h:linear_order α] : has_le (buffer α) := ⟨buffer.le⟩
+
+instance decidable_le {α} [h:linear_order α] [r:decidable_rel (h.lt)]
+: Π(x y : buffer α), decidable (x ≤ y)
+| ⟨m,a⟩ ⟨n,b⟩ :=
+begin
+  simp [has_le.le, buffer.le],
+  apply_instance,
+end
+
+protected
+def lt {α} [h:linear_order α] : buffer α → buffer α → Prop
+| ⟨m,a⟩ ⟨n,b⟩ := array.lex_lt a b
+
+instance {α} [h:linear_order α] : has_lt (buffer α) := ⟨buffer.lt⟩
+
+instance decidable_lt {α} [h:linear_order α] [r:decidable_rel (h.lt)]
+: Π(x y : buffer α), decidable (x < y)
+| ⟨m,a⟩ ⟨n,b⟩ :=
+begin
+  simp [has_lt.lt, buffer.lt],
+  apply_instance,
+end
+
+/- Slice a buffer. -/
+def slice {α} : Π(a : buffer α) (k l : ℕ) (k_le_l : k ≤ l), buffer α
+| ⟨n, a⟩ k l k_le_l :=
+  if l_lt_n : l ≤ n then
+    ⟨l - k, a.slice k l k_le_l l_lt_n⟩
+  else if p : k ≤ n then
+    ⟨n - k, a.slice k n p (nat.le_refl _)⟩
+  else
+    ⟨0, array.nil⟩
+
 end buffer
+
+namespace string
+
+/- Simplify functions calling through as_string -/
+theorem to_char_buffer_as_string (l:list char)
+: string.to_char_buffer (list.as_string l) = list.to_buffer l := eq.refl l.to_buffer
+
+end string
