lean/deps/typed_smt2/src/galois/sexpr.lean
@@ -4,6 +4,7 @@ expressions and reasoning about their interpretation.
 -/
 import system.io
 import data.array.lemmas -- from mathlib
+import galois.category.except
 
 import galois.data.array
 import galois.data.buffer
@@ -12,281 +13,32 @@ import galois.data.nat
 
 import .char_reader
 
-meta def dec_trivial_tac : tactic unit := do
-  tgt ← tactic.target,
-  let e := (`(@of_as_true) : expr) tgt,
-  r ← tactic.apply e,
-  tactic.exact `(trivial)
-
 universes u v w
+
+meta class has_to_expr (α : Type _) :=
+(to_expr : α → expr)
 
 /--
 Meta class for compile-time parsing of strings to data types.
 -/
-meta class is_meta_string (α : Type) :=
+meta class is_meta_string (α : Type) extends has_to_expr α :=
 (parse : string → except string α)
-(to_expr {} : α → tactic expr)
 
 /-- Tactic for constructing a term by parsing a string. -/
 meta def coerce (s:string) (α:Type) [is_meta_string α]  : tactic unit := do
   match is_meta_string.parse α s with
   | (except.ok r) := do
-    e ← is_meta_string.to_expr r,
-    tactic.exact e
+    tactic.exact (has_to_expr.to_expr r)
   | (except.error msg) := do
     tactic.fail msg
   end
 
+
 namespace sexpr
 
-namespace atom
-
-/-- Recognize legal characters in s-expressions. -/
-def is_legal_char (c:char) : Prop := not (c ∈ ['(', ')', ' ', '\t', '\n'])
-
-instance is_legal_char.decidable : decidable_pred is_legal_char :=
-begin
-  intro c,
-  unfold atom.is_legal_char,
-  apply_instance
-end
-
-theorem is_legal_digit_char (n:ℕ) : is_legal_char (nat.digit_char n) :=
-begin
-  unfold nat.digit_char,
-  by_cases (n =  0); simp only [h,if_pos, if_false], {dec_trivial_tac,},
-  by_cases (n =  1); simp only [h,if_pos, if_false], {dec_trivial_tac,},
-  by_cases (n =  2); simp only [h,if_pos, if_false], {dec_trivial_tac,},
-  by_cases (n =  3); simp only [h,if_pos, if_false], {dec_trivial_tac,},
-  by_cases (n =  4); simp only [h,if_pos, if_false], {dec_trivial_tac,},
-  by_cases (n =  5); simp only [h,if_pos, if_false], {dec_trivial_tac,},
-  by_cases (n =  6); simp only [h,if_pos, if_false], {dec_trivial_tac,},
-  by_cases (n =  7); simp only [h,if_pos, if_false], {dec_trivial_tac,},
-  by_cases (n =  8); simp only [h,if_pos, if_false], {dec_trivial_tac,},
-  by_cases (n =  9); simp only [h,if_pos, if_false], {dec_trivial_tac,},
-  by_cases (n = 10); simp only [h,if_pos, if_false], {dec_trivial_tac,},
-  by_cases (n = 11); simp only [h,if_pos, if_false], {dec_trivial_tac,},
-  by_cases (n = 12); simp only [h,if_pos, if_false], {dec_trivial_tac,},
-  by_cases (n = 13); simp only [h,if_pos, if_false], {dec_trivial_tac,},
-  by_cases (n = 14); simp only [h,if_pos, if_false], {dec_trivial_tac,},
-  by_cases (n = 15); simp only [h,if_pos, if_false], {dec_trivial_tac,},
-  dec_trivial_tac,
-end
-
-/-- Indicate if all characters in buffer are well-formed. -/
-def well_formed (b:char_buffer) : Prop
-  := ∀i, atom.is_legal_char (b.read i)
-  ∧ b ≠ buffer.nil
-
-namespace well_formed
-
-local attribute [reducible] well_formed
-instance decidable : decidable_pred well_formed := by apply_instance
-
-end well_formed
-end atom
-
-/-- This denotes an atom in the s-expression syntax.
-
-We have not done this yet, but we will need to adds
--/
-structure atom :=
-(to_char_buffer : char_buffer)
-(valid : atom.well_formed to_char_buffer)
-
-namespace atom
-
-protected def to_repr (a:atom) : string := a.to_char_buffer.to_string
-
-instance : has_repr atom := { repr := atom.to_repr }
-
-instance : decidable_eq atom := by tactic.mk_dec_eq_instance
-
-protected def lt (x y : atom) : Prop := x.to_char_buffer.to_string < y.to_char_buffer.to_string
-
-instance has_lt : has_lt atom := { lt := atom.lt }
-
-instance has_decidable_lt (x y : atom) : decidable (x < y) :=
-begin
-  simp [has_lt.lt, atom.lt],
-  apply_instance
-end
-
-/-- Map an s-expression to a meta-level expression -/
-protected
-meta def to_expr (c:atom) : tactic expr := do
-  let s := reflected.to_expr (string.reflect c.to_char_buffer.to_string),
-  let b := `(string.to_char_buffer %%s),
-  gs ← tactic.get_goals,
-  proof_var ← tactic.mk_meta_var `(atom.well_formed %%b),
-  tactic.set_goals [proof_var],
-  tgt ← tactic.target,
-  tactic.apply `(@of_as_true %%tgt),
-  success ← tactic.try_core (tactic.exact `(trivial)),
-  tactic.set_goals gs,
-  match success with
-  | option.none := tactic.fail $ repr c ++ " is an invalid s-expr atom."
-  | (option.some _):= do
-    pure `({ atom . to_char_buffer := %%b, valid := %%proof_var })
-  end
-
-@[simp]
-theorem size_push_back {α} (b:buffer α) (c:α)
-: (buffer.push_back b c).size = b.size + 1 :=
-begin
-  cases b,
-  trivial,
-end
-
-@[simp]
-theorem size_append_list {α} (b:buffer α) (l:list α)
-: (buffer.append_list b l).size = l.length + b.size :=
-begin
-  revert b,
-  induction l,
-  case list.nil {
-    intro b,
-    simp [buffer.append_list, nat.zero_add],
-  },
-  case list.cons : x r ind {
-    intro b,
-    simp only [buffer.append_list, ind, size_push_back, list.length_cons,
-               nat.add_succ, nat.add_zero, nat.succ_add],
-  },
-end
-
-theorem read_append_list_bound {α} {i:ℕ} {b:buffer α} {l:list α}
-: not (i < b.size)
-→ i < (buffer.append_list b l).size
-→ i - b.size < l.length :=
-begin
-  intros i_not_lt i_lt_append,
-  simp at i_not_lt,
-  simp only [size_append_list] at i_lt_append,
-  simp only [nat.sub_lt_to_add, i_lt_append, i_not_lt],
-  dec_trivial_tac,
-end
-
-/--
-This converts a nat to a char_buffer in decimal notation.
-
-Note. nat.repr seems to be builtin to the Lean VM magic, so it
-is much faster to invoke directly rather than using the functions
-used to define it.
--/
-protected def nat_to_decimal_buffer (n : ℕ) : char_buffer :=
-  n.repr.to_char_buffer
-
-
-/-- Show that decimal numbers will be well-formed atoms. -/
-theorem nat_to_decimal_buffer_is_well_formed (x:ℕ) : atom.well_formed (atom.nat_to_decimal_buffer x) :=
-begin
-  unfold atom.well_formed,
-
-  intro i_fin,
-  cases i_fin with i i_lt,
-  dsimp only [atom.nat_to_decimal_buffer],
-  dsimp only [nat.repr],
-  simp only [buffer.read_to_nth_le],
-  simp only [buffer.to_char_buffer_as_string],
-  apply and.intro,
-  -- Show repr only returns valid characters.
-  { simp only [buffer.to_list_to_buffer],
-    simp only [list.nth_le_reverse_simp],
-    simp only [list.nth_le_map'],
-    apply is_legal_digit_char
-  },
-  -- Show repr is non-empty
-  { apply mt (congr_arg buffer.to_list),
-    -- For some reason, the simplification rules below require ne is explicitly used
-    apply ne.elim,
-    simp only [buffer.to_list_to_buffer, buffer.nil_to_list],
-    -- The other rules work better with the ne eliminated.
-    simp only [ne, list.reverse_eq_nil],
-    simp only [list.map_eq_nil],
-    apply nat.to_digits_ne_nil,
-  },
-end
-
-/- Construct a atom from the decimal notation of a nat. -/
-def nat_to_decimal (x:ℕ) : atom := ⟨atom.nat_to_decimal_buffer x, atom.nat_to_decimal_buffer_is_well_formed x⟩
-
-end atom
-
-/--
-This is a data-structure for representing non-empty lists of
-well-formed s-expressions.  It does not allow dotted lists directly,
-and they would instead be parsed as a list with a dot followed by
-an atom.
-
-The term is structured to both simplify serialization and
-top-down/left-to-right parsing.
--/
-inductive sexpr_list : Type
-| atom : atom → sexpr_list
-| nil  : sexpr_list
-| parens : sexpr_list → sexpr_list
-| prepend_atom : atom → sexpr_list → sexpr_list
-| prepend_nil : sexpr_list → sexpr_list
--- @prepend_parens x y@ denotes @(x) y@.
-| prepend_parens : sexpr_list → sexpr_list → sexpr_list
-
-namespace sexpr_list
-
-protected
-def render {α} [has_append α] (rend : char_buffer → α) : sexpr_list → α
-| (atom b) := rend b.to_char_buffer
-| nil := rend "()".to_char_buffer
-| (parens s) := rend "(".to_char_buffer ++ (s.render ++ rend ")".to_char_buffer)
-| (prepend_atom b s) := rend b.to_char_buffer ++ (rend " ".to_char_buffer ++ s.render)
-| (prepend_nil s) := rend "() ".to_char_buffer ++ s.render
-| (prepend_parens p s) :=
-  rend "(".to_char_buffer ++ (p.render ++ (rend ") ".to_char_buffer ++ s.render))
-
-protected
-def to_repr (l:sexpr_list) : string := (sexpr_list.render id l).to_string
-
-/-- Return true if this is a single s-expression -/
-protected
-def is_single : sexpr_list → Prop
-| (atom _) := true
-| nil := true
-| (parens _) := true
-| (prepend_atom _ _) := false
-| (prepend_nil _) := false
-| (prepend_parens _ _) := false
-
-instance (e:sexpr_list) : decidable (e.is_single) :=
-begin
-  cases e; { unfold sexpr_list.is_single, apply_instance},
-end
-
-/-- Map an s-expression to a meta-level expression -/
-protected
-meta def to_expr : sexpr_list → tactic expr
-| (sexpr_list.atom a) := do
-  ae ← a.to_expr,
-  pure `(atom %%ae)
-| nil := do
-  pure `(nil)
-| (parens s) := do
-  e ← to_expr s,
-  pure `(parens %%e)
-| (prepend_atom a y) := do
-  ae ← a.to_expr,
-  e ← to_expr y,
-  pure `(prepend_atom %%ae %%e)
-| (prepend_nil y) := do
-  e ← to_expr y,
-  pure `(prepend_nil %%e)
-| (prepend_parens x y) := do
-  xe ← to_expr x,
-  ye ← to_expr y,
-  pure `(prepend_parens %%xe %%ye)
-
-instance : decidable_eq sexpr_list := by tactic.mk_dec_eq_instance
-
-end sexpr_list
+class is_atom (α : Type _) :=
+(to_char_buffer : α → char_buffer)
+(read {m} [char_reader string m] (n:ℕ) : m α)
 
 end sexpr
 
@@ -302,90 +54,77 @@ and two s expressions may be distinct, but render to the same string.
 The intent is to allow one to efficiently generate s-expressions,
 do lightweight pattern matching on them, and write them to handles.
 -/
-structure sexpr : Type :=
-(val  : sexpr.sexpr_list)
-(pr   : val.is_single)
+inductive sexpr (α:Type)
+| atom : α -> sexpr
+| parens : list sexpr -> sexpr
 
 namespace sexpr
 
 protected
-def mk_atom (c:atom) : sexpr := ⟨sexpr_list.atom c, by {unfold sexpr_list.is_single}⟩
+def mk_atom {α:Type} (c:α) : sexpr α := sexpr.atom c
 
 protected
-def nil : sexpr := ⟨sexpr_list.nil, by {unfold sexpr_list.is_single}⟩
-
-protected
-def parens (c:sexpr_list) : sexpr := ⟨sexpr_list.parens c, by {unfold sexpr_list.is_single}⟩
-
-namespace sexpr_list
-
-/-- Prepend sexpression to list -/
-def prepend : sexpr → sexpr_list → sexpr_list
-| ⟨sexpr_list.atom c, _⟩ y := prepend_atom c y
-| ⟨sexpr_list.nil,_⟩ y := prepend_nil y
-| ⟨sexpr_list.parens x, _⟩ y := prepend_parens x y
-
-end sexpr_list
-
-open sexpr_list
+def nil {α:Type} : sexpr α := sexpr.parens []
 
 /-- Render s-expression as a string -/
-protected def to_repr (s:sexpr) : string := s.val.to_repr
+mutual def render, list_render {α:Type} [h : is_atom α] {β} [has_append β] (rend : char_buffer → β)
+with render : sexpr α -> β
+     | (atom s) := rend (@is_atom.to_char_buffer _ h s)
+     | (parens []) := rend "()".to_char_buffer
+     | (parens (h::t)) := rend "(".to_char_buffer ++ render h ++ list_render t
+with list_render : list (sexpr α) -> β
+     | [] := rend ")".to_char_buffer
+     | (s :: ss) := rend " ".to_char_buffer ++ render s ++ list_render ss
 
-instance : has_repr sexpr :=
-{ repr := sexpr.to_repr }
+/-- Render s-expression as a string -/
+def repr {α:Type} [h : is_atom α] : sexpr α -> string := render buffer.to_string
 
+instance {α} [is_atom α] : has_repr (sexpr α) := { repr := sexpr.repr }
+
+/-- Construct an s-expression from a list of s-expressions -/
 protected
-def of_list_core : sexpr → list sexpr → sexpr_list
-| f [] := f.val
-| f (h::r) := prepend f (of_list_core h r)
-
-/-- Construct an s-expression from a list -/
-protected
-def of_list : list sexpr → sexpr
-| [] := sexpr.nil
-| (h::r) := sexpr.parens (sexpr.of_list_core h r)
-
-def read_atom {m} [char_reader string m] (n:ℕ) (b:char_buffer) : m atom := do
-  b1 ← char_reader.read_append_while atom.is_legal_char n b,
-  if h : atom.well_formed b1 then
-    pure ⟨b1, h⟩
-  else
-    throw $ repr b ++ " is not a valid atom."
-
+def of_list {α} : list (sexpr α) → sexpr α := sexpr.parens
 
 /-- A frame represents the first part of an s-expression that started with a open-paren -/
-structure frame :=
-(exprs : list sexpr)
+structure frame (α:Type) :=
+(exprs : list (sexpr α))
 
 namespace frame
 
 /-- Create an empty frame -/
-def nil : frame := ⟨[]⟩
+def nil {α} : frame α := ⟨[]⟩
 
 /-- Close a frame by appending close paren -/
-def close : frame → sexpr
-| ⟨[]⟩ := sexpr.nil
-| ⟨h::r⟩ := sexpr.parens (list.foldl (λx y, prepend y x) h.val r)
+def close {α} (f:frame α) : sexpr α := sexpr.parens f.exprs.reverse
 
 /-- This adds the partial token as an sexpression if the token is non-empty -/
-def append_sexpr (f:frame) (t:sexpr) : frame := ⟨ t :: f.exprs⟩
+def append_sexpr {α} (f:frame α) (t:sexpr α) : frame α := ⟨ t :: f.exprs⟩
 
 /-- This adds the partial token as an sexpression if the token is non-empty -/
-def append_frame (f:frame) (t:frame) : frame := ⟨ t.close :: f.exprs⟩
+def append_frame {α} (f:frame α) (t:frame α) : frame α := append_sexpr f t.close
 
 end frame
-
 
 section
 open char_reader
 
+/-- The character after an atom should be empty or a close paren or whitespace. -/
+def check_atom_term {m} [char_reader string m] : m unit := do
+  mc ← peek_char,
+ match mc with
+ | option.none := pure ()
+ | (option.some c) := do
+    when (c ∉ ['(', ')'] ∧ ¬c.is_whitespace)
+      (throw ("Unexpected character "++ c.repr)),
+    consume_char
+ end
+
 /-- Read the s-expression from the handle/ -/
-def read_core {m} [char_reader string m]
-  : ℕ → list frame → m sexpr
+def read_core {α:Type} [is_atom α] {m} [char_reader string m]
+  : ℕ → list (frame α) → m (sexpr α)
 | nat.zero frames := do
   throw "out of gas"
-| (nat.succ n) frames := do
+| (nat.succ n) frames := (do
   mc ← peek_char,
   match mc with
   | option.none :=
@@ -410,64 +149,70 @@ def read_core {m} [char_reader string m]
       consume_char,
       read_core n frames
     else do
-      consume_char,
-      a ← sexpr.mk_atom <$> read_atom n (buffer.nil.push_back c),
+      a ← sexpr.mk_atom <$> is_atom.read α n,
+      check_atom_term,
       match frames with
       | [] := pure a
       | (top_frame::lower_frames) := do
         read_core n (top_frame.append_sexpr a :: lower_frames)
       end
-  end
+  end)
 
 /-- Read the s-expression from the handle/ -/
-def read {m} [char_reader string m] (gas : ℕ) : m sexpr := do
-  read_core gas []
+def read (α:Type) [i:is_atom α] {m} [char_reader string m] (gas : ℕ) : m (sexpr α) :=
+  @read_core α i _ _ gas []
 
 end
 
-local attribute [instance] handle_char_reader.string_is_char_reader
+local attribute [instance] char_reader.handle_char_reader.string_is_char_reader
 
 /-- Read the s-expression from the handle/ -/
-def read_from_handle (h:io.handle) : io (except string sexpr) := do
+def read_from_handle {α} [i:is_atom α] (h:io.handle) : io (except string (sexpr α)) := do
   let gas : ℕ := 2^64-1 in
-  handle_char_reader.read_to_newline h (sexpr.read gas)
+  char_reader.read_from_handle h (@sexpr.read α i _ _ gas)
 
-local attribute [instance] string_char_reader.string_is_char_reader
+--local attribute [instance] string_char_reader.string_is_char_reader
 
-def parse (s:string) : except string sexpr :=
+/-- Parse the string as an s-expression -/
+def parse {α:Type} [i:is_atom α] (s:string) : except string (sexpr α) :=
   let gas : ℕ := 2^64-1 in
-  string_char_reader.read_to_end s (sexpr.read gas)
+  char_reader.read_from_string s (@sexpr.read α i _ _ gas)
 
-meta def to_expr : sexpr → tactic expr
-| ⟨sexpr_list.atom a,_⟩ := do
-   ae <- a.to_expr,
-   pure `(sexpr.mk_atom %%ae)
-| ⟨nil,_⟩ := do
-  pure `(sexpr.nil)
-| ⟨parens s, _⟩ := do
-  e ← s.to_expr,
-  pure `(sexpr.parens %%e)
+/-- Render s-expression as a string -/
+meta
+mutual def to_expr, list_to_expr {α:Type} [r:reflected α] [h:has_to_expr α]
+with to_expr : Π(s:sexpr α), expr
+     | (atom a) := `(@sexpr.atom α).to_expr.app (has_to_expr.to_expr a)
+     | (parens s) := `(@sexpr.parens α).to_expr.app (list_to_expr s)
+with list_to_expr  : Π(s:list (sexpr α)), expr
+     | [] := `(@list.nil α).to_expr
+     | (h :: t) := (`(@list.cons α).to_expr.subst (to_expr h)).subst (list_to_expr t)
 
-meta instance : is_meta_string sexpr :=
-{ parse := sexpr.parse
+
+meta instance (α:Type) [h:is_atom α] [reflected α] [has_to_expr α]
+: is_meta_string (sexpr α) :=
+{ parse := @sexpr.parse α h
 , to_expr := sexpr.to_expr
 }
 
 /-- Write the s-expression to the handle. -/
-def write (h:io.handle) (s:sexpr) : io unit :=
-  @sexpr_list.render (io unit) {append := λx y, x >> y} (io.fs.write h) s.val
+def write {α} [is_atom α] (h:io.handle) (s:sexpr α) : io unit :=
+  @sexpr.render α _ (io unit) {append := λx y, x >> y} (io.fs.write h) s
 
 local infixr  `<+>`:50 := sexpr.append
 
 -- Create an operation applied to some argumen  ts.
-def app (op:sexpr) (args : list sexpr) : sexpr := sexpr.parens (sexpr.of_list_core op args)
+def app {α} (op:sexpr α) (args : list (sexpr α)) : sexpr α :=
+  sexpr.parens (op :: args)
 
 /-- Apply an binary operation to two sexpressions. -/
-def bin_app (op:sexpr) (x y : sexpr) : sexpr :=
-  sexpr.parens (prepend op (prepend x y.val))
+def bin_app {α} (op:sexpr α) (x y : sexpr α) : sexpr α := sexpr.parens [op, x,y]
 
-def from_nat (n:ℕ) : sexpr := sexpr.mk_atom (atom.nat_to_decimal n)
+instance (α) [decidable_eq α] : decidable_eq (sexpr α) := by tactic.mk_dec_eq_instance
 
-instance : decidable_eq sexpr := by tactic.mk_dec_eq_instance
+/- Construct an atom from a string literal. -/
+def of_string {α} [i:is_atom α] (nm:string)
+      (p : except.is_ok (char_reader.read_from_string nm (@sexpr.read α i _ _ 1024)))
+: sexpr α := p.value
 
 end sexpr
