lean/deps/typed_smt2/src/galois/smt2/basic.lean
@@ -2,51 +2,560 @@
 This declares sorts, terms, and semantics for generating SMTLIB
 expressions and reasoning about their interpretation.
 -/
+import galois.data.buffer
+import galois.data.char
+import galois.data.fin
+import galois.data.nat
+import galois.logic
+
+import data.bitvec
+
 import galois.sexpr
+
+import tactic.find
 
 namespace smt2
 
-/-- This represents either function or sort symbol names. -/
-def symbol := sexpr.atom
+------------------------------------------------------------------------
+-- is_printable
 
-/-- Convert a symbol to an s-expression; this is currently unchecked. -/
-protected
-def symbol.to_sexpr (s:symbol) : sexpr := sexpr.mk_atom s
+/-- Predicate that holds if character is considered an SMTLIB printable character. -/
+def is_printable (c:char) : Prop := 0x20 ≤ c.val ∧ c.val ≠ 127
+
+namespace is_printable
+local attribute [reducible] is_printable
+instance decidable_is_printable (c:char) : decidable (is_printable c) := by apply_instance
+end is_printable
+
+theorem alpha_is_printable {c:char} : c.is_alpha → is_printable c :=
+begin
+  unfold char.is_alpha, unfold is_printable,
+  intro isa,
+  cases isa;
+  {
+    simp [char.is_upper, char.is_lower] at isa,
+    apply and.intro,
+    { transitivity, tactic.swap, exact isa.left, exact dec_trivial, },
+    { intro eq,
+      simp [eq] at isa,
+      exact  of_as_false isa trivial,
+    }
+  },
+end
+
+theorem digit_is_printable {c:char} : c.is_digit → is_printable c :=
+begin
+  unfold char.is_digit, unfold is_printable,
+  intro isd,
+  apply and.intro,
+  { transitivity, tactic.swap, exact isd.left, exact dec_trivial, },
+  { intro eq,
+    simp [eq] at isd,
+    exact  of_as_false isd trivial,
+  },
+end
+
+------------------------------------------------------------------------
+-- is_legal
+
+/-- Legal characters are either printable characters or whitespace. -/
+def is_legal (c:char) : Prop := is_printable c ∨ c ∈ ['\t', '\n', '\x0d']
+
+namespace is_legal
+local attribute [reducible] is_legal
+instance is_legal_decidable (c:char) : decidable (is_legal c) := by apply_instance
+
+end is_legal
+
+------------------------------------------------------------------------
+-- reserved_words
+
+/--
+This is the list of reserved words in SMTLIB.
+
+TODO: Add all commands in Section 3.9
+-/
+def reserved_words : list string :=
+  [ "BINARY"
+  , "DECIMAL"
+  , "HEXADECIMAL"
+  , "NUMERAL"
+  , "STRING"
+  , "_"
+  , "!"
+  , "as"
+  , "let"
+  , "exists"
+  , "forall"
+  , "match"
+  , "par"
+  ]
+
+def reserved_word := { s:string // s ∈ reserved_words }
+
+instance reserved_word.repr : has_repr reserved_word := ⟨subtype.val⟩
+
+/--
+Construct a reserved word from a character buffer using the decidability of reserved word membership.
+-/
+def reserved_word.mk (s:string) (p:as_true (s ∈ reserved_words)) : reserved_word := ⟨s, of_as_true p⟩
+
+
+/-- Reserved words as a list of character buffers. -/
+def reserved_words_buffer : list char_buffer := reserved_words.map string.to_char_buffer
+
+/-- Return true if buffer is a reserved word. -/
+def is_reserved_word (b:char_buffer) : Prop :=
+  b ∈ reserved_words_buffer
+
+namespace is_reserved_word
+local attribute [reducible] is_reserved_word
+instance decidable : decidable_pred is_reserved_word := by apply_instance
+end is_reserved_word
+
+------------------------------------------------------------------------
+-- symbol
 
 namespace symbol
 
-/--
-Return true if this symbol is a legal name.
+/-- Check character is allowed in a symbol. -/
+def is_symbol_char (c:char) : Prop := is_legal c ∧ c ∉ ['|', '\\']
 
-TODO: Fix this to ensure symbol is not a reserved word, and characters are valid.
--/
-def is_valid (nm:symbol) : bool := tt
+namespace is_symbol_char
+local attribute [reducible] is_symbol_char
+instance decidable : decidable_pred is_symbol_char := by apply_instance
+end is_symbol_char
 
-instance : has_lt symbol :=
+/-- A simple symbol character is a quoted symbol. -/
+theorem digit_is_symbol_char {c:char}
+: char.is_digit c → is_symbol_char c :=
 begin
-  unfold symbol,
-  apply_instance
+  intro h,
+  unfold is_symbol_char,
+  unfold is_legal,
+  apply and.intro,
+  exact or.inl (digit_is_printable h),
+  { intro p, simp at p,
+    cases p; simp only [p] at h; exact (of_as_false h trivial),
+  },
 end
 
-instance : has_repr symbol := { repr := λs, s.to_repr }
+/-- Check all characters in buffer can appear in quoted symbols. -/
+def is_symbol (b:char_buffer) : Prop
+  := ∀(i: fin b.size), is_symbol_char (b.read i)
+
+namespace is_symbol
+local attribute [reducible] is_symbol
+instance decidable : decidable_pred is_symbol := by apply_instance
+end is_symbol
 
 end symbol
 
-/-- A type for terms in SMTLIB -/
-def sort : Type := sexpr
+/-- This is a simple identifier that can be used in function or symbol names. -/
+structure symbol :=
+(to_char_buffer : char_buffer)
+(valid : symbol.is_symbol to_char_buffer)
 
+namespace symbol
+
+instance decidable_eq : decidable_eq symbol := by tactic.mk_dec_eq_instance
+
+protected def le (x y : symbol) : Prop := x.to_char_buffer ≤ y.to_char_buffer
+instance : has_le symbol := ⟨symbol.le⟩
+instance decidable_le
+: Π(x y : symbol), decidable (x ≤ y)
+| ⟨m,a⟩ ⟨n,b⟩ :=
+begin
+  simp [has_le.le, symbol.le],
+  apply_instance,
+end
+
+protected def lt (x y : symbol) : Prop := x.to_char_buffer < y.to_char_buffer
+instance : has_lt symbol := ⟨symbol.lt⟩
+instance decidable_lt
+: Π(x y : symbol), decidable (x < y)
+| ⟨m,a⟩ ⟨n,b⟩ :=
+begin
+  simp [has_lt.lt, symbol.lt],
+  apply_instance,
+end
+
+section simple_symbols
+
+/-- Symbol characters allowed in simple symbols -/
+def simple_char_symbols : list char :=
+ ['~', '!', '@', '$', '%', '^', '&', '*', '_', '-', '+', '=', '<', '>', '.', '?', '/' ]
+
+/-- Predicate that checks if character is allowed in a simple symbol. -/
+inductive is_simple_symbol_char (c:char) : Prop
+| is_alpha : char.is_alpha c → is_simple_symbol_char
+| is_digit : char.is_digit c → is_simple_symbol_char
+| is_other : c ∈ simple_char_symbols → is_simple_symbol_char
+
+-- Show is_simple_symbol_char is decidable.
+open is_simple_symbol_char
+
+open decidable
+
+instance is_simple_symbol_char.decidable : decidable_pred is_simple_symbol_char
+| c :=
+  if f : c.is_alpha then
+    is_true (is_alpha f)
+  else if g : c.is_digit then
+    is_true (is_digit g)
+  else if h : c ∈ simple_char_symbols  then
+    is_true (is_other h)
+  else
+    is_false begin intro p, cases p; contradiction, end
+
+/-- A simple symbol character is a quoted symbol. -/
+theorem is_simple_symbol_char.is_symbol_char {c:char}
+: is_simple_symbol_char c → is_symbol_char c :=
+begin
+  intro h,
+  cases h,
+  case is_simple_symbol_char.is_alpha : h {
+    unfold is_symbol_char,
+    unfold is_legal,
+    apply and.intro,
+    exact or.inl (alpha_is_printable h),
+    { intro p, simp at p,
+      cases p; simp only [p] at h; exact (of_as_false h trivial),
+    },
+  },
+  case is_simple_symbol_char.is_digit : h {
+    exact digit_is_symbol_char h,
+  },
+  case is_simple_symbol_char.is_other : h {
+    simp [simple_char_symbols] at h,
+    -- Try all characters and show they are allowed.
+    iterate { cases h, simp only [h], exact (of_as_true trivial), },
+  },
+end
+
+/-- Return true if this is a valid simple symbol. -/
+def is_simple_symbol (b:char_buffer) : Prop
+  := b ≠ buffer.nil
+  ∧ ¬(is_reserved_word b)
+  ∧ ∀(i: fin b.size),
+     let c := b.read i
+      in is_simple_symbol_char c ∧ (i.val = 0 → ¬(c.is_digit))
+
+local attribute [reducible] is_simple_symbol
+instance is_simple_symbol.decidable : decidable_pred is_simple_symbol := by apply_instance
+
+end simple_symbols
+
+------------------------------------------------------------------------
+-- repr
+
+section repr
+
+/-- Render a symbol as a simple symbol is possible and quoted symbol otherwise. -/
+protected
+def repr (s:symbol) : string :=
+  if is_simple_symbol s.to_char_buffer then
+    s.to_char_buffer.to_string
+  else
+    "|" ++ s.to_char_buffer.to_string ++ "|"
+
+instance : has_repr symbol := ⟨symbol.repr⟩
+
+end repr
+
+------------------------------------------------------------------------
+-- Parsing
+
+section parsing
+
+theorem simple_symbol_is_symbol {b:char_buffer} : is_simple_symbol b → is_symbol b := do
+begin
+  simp [is_simple_symbol, is_symbol],
+  intros is_not_nil is_not_reserved char_pred,
+  intro i,
+  let p : is_simple_symbol_char (buffer.read b i) := (char_pred i).left,
+  exact (is_simple_symbol_char.is_symbol_char p),
+end
+
+/--
+A quoted symbol with the form "|???|" where '???' denotes
+a list of legal characters '|' and '\\'.
+-/
+def is_quoted_symbol (b:char_buffer) : Prop
+  := b.size ≥ 2
+  ∧ ∀(i: fin b.size),
+    if i.val = 0 ∨ i.val = b.size - 1 then
+      b.read i = '|'
+    else
+      is_symbol_char (b.read i)
+
+local attribute [reducible] is_quoted_symbol
+instance is_quoted_symbol.decidable : decidable_pred is_quoted_symbol := by apply_instance
+
+/- This parses the string as a symbol -/
+protected
+def parse (s:string) : except string symbol := do
+  let b := s.to_char_buffer,
+  if p:is_simple_symbol b then
+    pure ⟨b, simple_symbol_is_symbol p⟩
+  else if is_quoted_symbol b then (do
+    let inner : char_buffer := (b.take (b.size - 1)).drop 1,
+    if valid:is_symbol inner then
+      pure ⟨inner, valid⟩
+    else
+      throw "internal symbol parsing inconsistency")
+  else
+    throw "Invalid symbol"
+
+end parsing
+
+
+/--
+Construct a reserved word from a character buffer using the decidability of reserved word membership.
+-/
+def from_decidable (s:char_buffer) (p:as_true (is_symbol s)) : symbol := ⟨s, of_as_true p⟩
+
+/-- Map an s-expression to a meta-level expression -/
+protected
+meta def to_expr : symbol → expr
+| ⟨b, p⟩ := do
+  let s : string := b.to_string,
+  let r : reflected _ := `(from_decidable),
+  let f : expr := (`(string.to_char_buffer) : expr).app `(s),
+  ((r : expr).app f).app `(trivial)
+
+meta instance : is_meta_string symbol :=
+{ parse := symbol.parse
+, to_expr := symbol.to_expr
+}
+
+/- Construct an atom from a string literal. -/
+def of_string : Π(nm:string), (symbol.parse nm).is_ok → symbol
+| _ p := p.value
+
+theorem is_symbol_append {x y : char_buffer}
+: is_symbol x → is_symbol y → is_symbol (x ++ y) :=
+begin
+
+  unfold is_symbol,
+  intros p q i,
+  simp only [buffer.read_append],
+  apply (dite (i.val < buffer.size x)),
+  {
+    intro i_lt,
+    simp [i_lt],
+    exact (p _),
+  },
+  {
+    intro i_ge,
+    simp [i_ge],
+    exact (q _),
+  }
+end
+
+protected def append : symbol → symbol → symbol
+| ⟨x,p⟩ ⟨y,q⟩ := ⟨x ++ y, is_symbol_append p q⟩
+
+instance : has_append symbol := ⟨symbol.append⟩
+
+theorem is_symbol_nat (v : ℕ) : is_symbol (string.to_char_buffer (repr v)) :=
+begin
+  unfold is_symbol,
+
+  intro i_fin,
+  cases i_fin with i i_lt,
+  simp only [buffer.read_to_nth_le],
+
+  simp only [repr, has_repr.repr, nat.repr],
+  simp only [buffer.to_char_buffer_as_string],
+  simp only [buffer.to_list_to_buffer],
+
+  simp only [list.nth_le_reverse_simp],
+  simp only [list.nth_le_map'],
+
+  apply digit_is_symbol_char,
+  apply char.digit_char_is_digit,
+  exact (nat.nth_to_digits_is_lt (of_as_true trivial) _),
+end
+
+/- Construct an atom from a string literal. -/
+def of_nat (v : ℕ) : symbol := ⟨string.to_char_buffer (repr v), is_symbol_nat v⟩
+
+def of_prefixed_nat (pre:string) (p : (symbol.parse pre).is_ok) (v : ℕ) : symbol :=
+  of_string pre p ++ of_nat v
+
+end symbol
+
+------------------------------------------------------------------------
+-- atom
+
+/- A atomic expression within an SMTLIB s-expression. -/
+inductive atom
+| reserved_word (b:char_buffer) : is_reserved_word b → atom
+| symbol : symbol → atom
+| numeral : ℕ → atom
+
+namespace atom
+
+protected
+def repr : atom → string
+| (reserved_word b _) := b.to_string
+| (symbol s)   := s.repr
+| (numeral s)  := s.repr
+
+protected
+def to_char_buffer : atom → char_buffer
+| (reserved_word b _) := b
+| (symbol s)  := s.repr.to_char_buffer
+| (numeral s) := s.repr.to_char_buffer
+
+protected
+def read {m} [char_reader string m] (read_count:ℕ) : m atom := do
+  mc ← char_reader.peek_char,
+  match mc with
+  | option.none := throw "Dog Unexpected end of stream."
+  | option.some '|' := do
+    char_reader.consume_char,
+    b ← char_reader.read_while symbol.is_symbol_char read_count,
+    last_char ← char_reader.read_char,
+    (when (last_char ≠ '|') $
+      throw ("Unexpected character " ++ repr last_char ++ "in quoted symbol.")),
+    if valid:symbol.is_symbol b then
+      pure (symbol ⟨b, valid⟩)
+    else
+      throw $ "Invalid symbol " ++ repr b
+  | option.some c :=
+    if c.is_digit then (do
+      b ← char_reader.read_while char.is_digit read_count,
+      pure (numeral b.to_string.to_nat))
+    else if symbol.is_simple_symbol_char c then (do
+      -- Read symbol characters
+      b ← char_reader.read_while symbol.is_simple_symbol_char read_count,
+      if is_res:is_reserved_word b then
+        pure (reserved_word b is_res)
+      else if valid:symbol.is_simple_symbol b then
+        pure (symbol ⟨b, symbol.simple_symbol_is_symbol valid⟩)
+      else
+        throw $ "Invalid symbol " ++ repr b)
+    else
+      throw $ "Unexpected character " ++ repr c
+  end
+
+instance : sexpr.is_atom atom :=
+{ to_char_buffer := atom.to_char_buffer
+, read := @atom.read
+}
+
+/-
+protected
+meta def to_expr : atom → expr
+| (symbol s) := `(symbol).to_expr.app s.to_expr
+| (numeral n) := `(numeral).to_expr.app (reflect n).to_expr
+
+
+meta instance has_to_expr_atom : has_to_expr atom := ⟨atom.to_expr⟩
+-/
+
+/- Construct an atom from a string literal. -/
+def of_string : Π(nm:string), (char_reader.read_from_string nm (@atom.read _ _ nm.length)).is_ok → atom
+| _ p := p.value
+
+instance : has_coe atom (sexpr atom) := ⟨sexpr.atom⟩
+
+end atom
+
+namespace symbol
+
+/-- Construct an atom from an s-expression. -/
+def to_sexpr (s:symbol) : sexpr atom := sexpr.atom (atom.symbol s)
+
+instance : has_coe symbol (sexpr atom) := ⟨to_sexpr⟩
+
+end symbol
+
+------------------------------------------------------------------------
+-- identifier
+
+namespace identifier
+
+/- An argument to an identifier. -/
+inductive index
+| numeral : ℕ → index
+| symbol : symbol → index
+
+namespace index
+
+instance : decidable_eq index := by tactic.mk_dec_eq_instance
+
+protected def to_atom : index → atom
+| (numeral n) := atom.numeral n
+| (symbol s)  := atom.symbol s
+
+protected def to_sexpr (i:index) : sexpr atom := sexpr.atom i.to_atom
+
+end index
+
+instance coe_nat_to_index : has_coe ℕ index := ⟨index.numeral⟩
+instance coe_symbol_to_index : has_coe symbol index := ⟨index.symbol⟩
+
+end identifier
+
+/- An identifier in SMTLIB possibly with a list of indices as arguments. -/
+structure identifier :=
+(head : symbol)
+(indices : list identifier.index)
+
+namespace identifier
+
+instance : decidable_eq identifier := by tactic.mk_dec_eq_instance
+
+protected
+def to_sexpr : identifier → sexpr atom
+| ⟨s, []⟩ := s.to_sexpr
+| ⟨s, l⟩  := sexpr.parens (sexpr.of_string "_" trivial :: s :: (index.to_sexpr <$> l))
+
+instance : has_coe identifier (sexpr atom) := ⟨identifier.to_sexpr⟩
+
+end identifier
+
+------------------------------------------------------------------------
+-- sort
+
+/-- A type for terms in SMTLIB -/
+def sort : Type := identifier
+
+namespace sort
 instance : decidable_eq sort := by { unfold sort, apply_instance }
 
+protected
+def to_sexpr : sort → sexpr atom := identifier.to_sexpr
+
+instance sort_is_sexpr : has_coe sort (sexpr atom) := ⟨sort.to_sexpr⟩
+
+end sort
+
 /-- Denotes Booleans -/
-def bool : sort := (by coerce "bool" sexpr)
+def bool : sort := ⟨symbol.of_string "bool" trivial, []⟩
+
+------------------------------------------------------------------------
+-- inhabited_type
 
 /-- A type with a default value in that type. -/
 structure inhabited_type :=
 (type : Type)
 (value : type)
 
+namespace inhabited_type
+
+def bool : inhabited_type := { type := Prop, value := true }
+
 /-- A type with natural numbers that can be used for uninterpreted values. -/
-def inhabited_type.uninterpreted : inhabited_type := { type := ℕ, value := 0 }
+def uninterpreted : inhabited_type := { type := ℕ, value := 0 }
+
+end inhabited_type
+
+------------------------------------------------------------------------
+-- logic
 
 /--
 This defines an interpretation of sorts.
@@ -62,33 +571,35 @@ We use a function rather than finite map to deal with polymorphic
 types such as bitvectors.
 -/
 structure logic :=
-(eval : sort → inhabited_type)
-(bool_eqn : (eval bool).type = Prop)
+(interpretation : sort → inhabited_type)
+(bool_correct : (interpretation bool).type = Prop)
 
 namespace logic
 
-/-- Return the type associated with the given sort or Prop if not defined -/
-def type_of (l:logic) (s:sort) : Type := (l.eval s).type
+--- Return the type associated with the given sort or Prop if not defined
+def type_of (l:logic) (s:sort) : Type := (l.interpretation s).type
 
-/-- Assert proposition is assigned to Booleans -/
-def prop_is_bool_type (l:logic) : l.type_of bool = Prop := l.bool_eqn
+-- Assert proposition is assigned to Booleans
+--def prop_is_bool_type (l:logic) : l.type_of bool = inhabited_type.bool := l.bool_correct
 
-/-- Return the type associated with the given sort or Prop if not defined -/
-def value_of (l:logic) (s:sort) : l.type_of s := (l.eval s).value
+/-- Coercision from prop to l.type_of bool -/
+def of_prop (l:logic) (x:Prop) : l.type_of bool := cast (eq.symm l.bool_correct) x
+
+/-- Coercision from prop to l.type_of bool -/
+def to_prop (l:logic) (x:l.type_of bool) : Prop := cast l.bool_correct x
 
 /-- @fun_type args res@ dReturn the type assigned to functions. -/
 def fun_domain (l:logic) : list sort → sort → Type
 | [] res := l.type_of res
-| (h::r) tp := l.type_of h → fun_domain r tp
+| (h::r) s := l.type_of h → fun_domain r s
 
-/-- Default value for a function -/
+--- Return the type associated with the given sort or Prop if not defined
+def value_of (l:logic) (s:sort) : l.type_of s := (l.interpretation s).value
+
+--- Default value for a function
 def fun_default_value (l:logic) : Π(args:list sort) (res:sort), l.fun_domain args res
 | [] res := l.value_of res
 | (h::r) tp := λ(x : l.type_of h), fun_default_value r tp
-
-/-- Coercision from prop to l.type_of bool -/
-instance bool_coe (l:logic) : has_coe Prop (l.type_of bool) :=
-{ coe := λ(x:Prop), eq.rec x l.prop_is_bool_type.symm }
 
 end logic
 
@@ -107,6 +618,72 @@ def model (l:logic) : Type := rbmap symbol (Σ(args:list sort) (s:sort), l.fun_d
 instance (l:logic) : has_emptyc (model l) :=
 { emptyc := mk_rbmap _ _ }
 
+namespace model
+
+section
+parameter {l:logic}
+
+/-- Bind a function to symbol name in the module. -/
+def bind (ctx:model l)  (nm:symbol) {args: list sort} {r:sort} (v:l.fun_domain args r) : model l :=
+  ctx.insert nm ⟨args, r, v⟩
+
+/-- Bind a constant to a symbol name in the module. -/
+def bind_const (ctx:model l) (nm:symbol) {r:sort} (v:l.type_of r) : model l :=
+  @bind ctx nm [] r v
+end
+end model
+
+------------------------------------------------------------------------
+-- evaluator
+
+namespace evaluator
+
+/-- Errors thrown during evaluation. -/
+inductive error
+| var_undefined (nm:symbol) : error
+| incorrect_var_result_sort (nm:symbol) {defined read:sort} (ineq:defined ≠ read) : error
+| incorrect_var_arg_sorts (nm:symbol) {defined read : list sort} (ineq:defined ≠ read) : error
+
+end evaluator
+
+
+def evaluator := except evaluator.error
+
+namespace evaluator
+local attribute [reducible] evaluator
+instance : monad evaluator := by apply_instance
+instance : monad_except error evaluator := by apply_instance
+
+/-
+instance (l:logic) : monad_reader (model l) (evaluator l) := by apply_instance
+protected
+def run {l} {α} (m:evaluator l α) (mdl:model l) : except evaluator.error α := m.run mdl
+-/
+
+end evaluator
+
+namespace model
+
+/-- Return the value associated with a symbol, or a default value if not defined. -/
+def symbol_value {l:logic} (m:model l) (nm:symbol) (args:list sort) (res:sort)
+: evaluator (l.fun_domain args res) :=
+  match rbmap.find m nm with
+  | option.none := throw (evaluator.error.var_undefined nm)
+  | option.some ⟨nm_args, nm_res, nm_val⟩ :=
+    if arg_eq : nm_args = args then
+      if res_eq : nm_res = res then
+        pure (eq.rec (eq.rec nm_val arg_eq) res_eq)
+      else
+        throw (evaluator.error.incorrect_var_result_sort nm res_eq)
+     else
+        throw (evaluator.error.incorrect_var_arg_sorts nm arg_eq)
+  end
+
+end model
+
+------------------------------------------------------------------------
+-- term
+
 /--
 A term in SMTLIB representation.
 
@@ -120,61 +697,48 @@ can give an incorrect interpretation to an expression.
 We recommend users only construct terms manually if they must, and
 otherwise use existing definitions.
 -/
-structure term (s : sort) :=
-(repr : sexpr)
-(interp : Π{l:logic}, model l → l.type_of s)
+structure term (l:logic) (s : sort) :=
+(repr : sexpr atom)
+(interp : model l → l.type_of s)
 
 namespace model
-
-section
-parameter {l:logic}
-
-/-- Bind a function to symbol name in the module. -/
-def bind (ctx:model l)  (nm:symbol) {args: list sort} {r:sort} (v:l.fun_domain args r) : model l :=
-  ctx.insert nm ⟨args, r, v⟩
-
-/-- Bind a constant to a symbol name in the module. -/
-def bind_const (ctx:model l)  (nm:symbol) {r:sort} (v:l.type_of r) : model l :=
-  @bind ctx nm [] r v
-
-/-- Return the value associated with a symbol, or a default value if not defined. -/
-def symbol_value (m:model l) (nm:symbol) (args:list sort) (res:sort) : l.fun_domain args res :=
-  match rbmap.find m nm with
-  | option.none := l.fun_default_value args res
-  | option.some ⟨nm_args, nm_res, nm_val⟩ :=
-    if h : nm_args = args ∧ nm_res = res then
-      eq.rec (eq.rec nm_val h.left) h.right
-     else
-      l.fun_default_value args res
-  end
 
 /-- @mdl.fun_value args rhs@ returns the value associated with a
 function that takes the given  arguments and returns the value denoted by @rhs@.
 -/
 def fun_value {l:logic}
-: Π(mdl : model l) (args : list (symbol × sort)) {res : sort} (rhs : term res),
+: Π(mdl:model l) (args : list (symbol × sort)) {res : sort} (rhs : term l res),
    l.fun_domain (args.map prod.snd) res
 | mdl [] res rhs := rhs.interp mdl
-| mdl (⟨nm,s⟩::args) res rhs := λ(x:l.type_of s), (mdl.bind_const nm x).fun_value args rhs
+| mdl (⟨nm,s⟩::args) res rhs := (λ(x:l.type_of s), fun_value (mdl.bind_const nm x) args rhs)
 
-end
 end model
 
-section term
+
+namespace term
+
+
+instance (l:logic) (s:sort) : has_coe (term l s) (sexpr atom) := ⟨term.repr⟩
+
+end term
 
 /-- Create a term from a  symbol and sort -/
-def var (nm : symbol) {s:sort} : term s :=
+def var {l:logic} (nm : symbol) (s:sort) : term l s :=
 { repr := nm.to_sexpr
-, interp := λ_ m, m.symbol_value nm [] s
+, interp := λ(m:model l),
+   match m.symbol_value nm [] s with
+   | (except.ok r) := r
+   | (except.error e) := l.value_of s
+   end
 }
 
 /-- Generate term that two terms are equal. -/
-def eq {s:sort} (x y : term s) : term bool :=
-{ repr := sexpr.bin_app (by coerce "=" sexpr) x.repr y.repr
-, interp := λ_ m, x.interp m = y.interp m
+protected
+def eq {l:logic} {s:sort} (x y : term l s) : term l bool :=
+{ repr := sexpr.bin_app (sexpr.of_string "=" trivial) x.repr y.repr
+, interp := λmdl, l.of_prop (x.interp == y.interp)
 }
 
-end term
 
 ------------------------------------------------------------------------
 -- Additional data types
@@ -189,5 +753,16 @@ inductive literal
 | is_true : symbol → literal
 -- Assertion named predicate is false.
 | is_false : symbol → literal
+
+------------------------------------------------------------------------
+-- string_literal
+
+/-- Return true if each character is legal in a string lit. -/
+def is_string_lit_char (c:char)
+  := c.is_ascii7_printable
+  ∨ c ∈ ['\t', '\n', char.of_nat 13]
+
+def is_string_lit (b:char_buffer) : Prop :=
+  ∀(i:fin b.size), is_string_lit_char (b.read i)
 
 end smt2
