lean/deps/galois_stdlib/src/galois/data/array.lean
@@ -1,6 +1,35 @@
+-- Additional definitions for arrays
+import data.array.lemmas
 
+import .array.lex_order
+
+import ..logic
+
+import tactic.find
 
 namespace array
+
+/- Simplification rule for reading from an array constructed by push_back with a less-than test. -/
+theorem read_push_back_lt_iff {α} {n:ℕ} (a : array n α) (x:α) (i : fin (n+1))
+: read (push_back a x) i =
+  if lt:i.val < n then
+    read a ⟨i.val,lt⟩
+  else
+    x :=
+begin
+ cases i with i i_lt_plus_1,
+ have i_le := nat.le_of_succ_le_succ i_lt_plus_1,
+ dsimp [push_back, read, d_array.read],
+ cases (decide (i = n)),
+ case decidable.is_true  : is_eq {
+   simp [is_eq],
+ },
+ case decidable.is_false : is_neq {
+   have i_lt := lt_of_le_of_ne i_le is_neq,
+   simp [is_neq, i_lt],
+ },
+end
+
 
 /-- Empty buffer converted to array is same as array.nil -/
 @[simp]
