lean/deps/galois_stdlib/src/galois/data/nat/basic.lean
@@ -1,0 +1,79 @@
+import data.nat.basic
+
+-- This  file contains basic lemmas for nat
+namespace nat
+
+/-- pred _ + _ rewrite rule. -/
+theorem pred_add (m n : ℕ) : pred m + n = if m = 0 then n else pred (m + n) :=
+begin
+  cases m,
+  case zero {
+    simp,
+  },
+  case succ : m {
+    have p : ¬(succ m = 0) := by trivial,
+    simp [pred, p],
+  },
+end
+
+/-- _ + pred _ rewrite rule. -/
+theorem add_pred (m n : ℕ) : m + pred n = if n = 0 then m else pred (m + n) :=
+begin
+  cases n,
+  case zero {
+    simp,
+  },
+  case succ : n {
+    have p : ¬(succ n = 0) := by trivial,
+    simp [pred, p],
+  },
+end
+
+-- Reduce x < y to theorem with addition
+protected theorem lt_is_succ_le (x y : ℕ) : x < y ↔ x + 1 ≤ y := by trivial
+
+-- Reduce succ x < succ y
+protected lemma succ_lt_succ_iff : ∀{m n : ℕ}, succ n < succ m ↔ n < m :=
+begin
+  intros m n,
+  simp [nat.lt_is_succ_le, succ_le_succ_iff],
+end
+
+-- This rewrites a subtraction on left-hand-side of inequality into a predicate
+-- involving addition.
+protected lemma sub_lt_to_add (a m n : ℕ) : a - n < m ↔ (a < m + n ∧ (n ≤ a ∨ 0 < m)) :=
+begin
+  revert a m,
+  induction n,
+  case zero {
+    intros a m,
+    simp [zero_le],
+  },
+  case succ : n ind {
+    intros a m,
+    cases a,
+    case zero {
+      simp [zero_sub, zero_lt_succ, not_succ_le_zero],
+    },
+    case succ {
+      simp [add_succ, nat.succ_lt_succ_iff, succ_le_succ_iff, ind],
+    },
+  },
+end
+
+-- This rewrites a subtraction on right-hand side of inequality into an addition.
+protected lemma lt_sub_iff (a m n : ℕ) : a < m - n ↔ a + n < m :=
+begin
+  revert n,
+  induction m with m ind,
+  { simp [nat.lt_is_succ_le, add_succ, not_succ_le_zero, zero_sub],
+  },
+  { intro n,
+    cases n with n,
+    { simp, },
+    { simp [nat.succ_lt_succ_iff, ind],
+    },
+  },
+end
+
+end nat
