lean/deps/galois_stdlib/src/galois/logic.lean
@@ -1,0 +1,11 @@
+-- Definitions
+
+--- Use type-class resolution to find a decidable instance.
+def decide (p:Prop) [h:decidable p] : decidable p := h
+
+
+--- Use decidable instance to prove any theorem is we have a proof of the theorem, but it is false.
+theorem  of_as_false {P : Prop} [h:decidable P] (p:P) (q : as_false P) {α : Prop} : α :=
+begin
+  simp [as_false] at q, contradiction,
+end
