lean/deps/typed_smt2/src/galois/smt2/cmd.lean
@@ -1,0 +1,44 @@
+import .basic
+
+namespace smt2
+
+/-- An SMT command -/
+structure cmd :=
+(expr : sexpr atom)
+
+namespace cmd
+
+/-- Write command to a handle. -/
+protected
+def write (c:cmd) (h:io.handle) : io punit := sexpr.write h (c.expr)
+
+/-- Construct assert command. -/
+protected
+def assert {l} (p:term l bool) : cmd := ⟨sexpr.app (sexpr.of_string "assert" trivial) [p]⟩
+
+/-- Construct check-sat command. -/
+protected
+def check_sat : cmd := ⟨sexpr.parens [sexpr.of_string "check-sat" trivial]⟩
+
+/-- Declare a constant -/
+protected
+def declare_const (nm:symbol) (res:sort) : cmd :=
+  ⟨sexpr.app (sexpr.of_string "declare-const" trivial) [nm, res]⟩
+
+/-- Declare a function -/
+protected
+def declare_fun (nm:symbol) (args:list sort) (res:sort) : cmd :=
+  ⟨sexpr.app (sexpr.of_string "declare-fun" trivial) [nm, sexpr.parens (args.map sort.to_sexpr), res]⟩
+
+/-- Map a symbol and sort pair from a function declaration to an s-expression -/
+def arg_pair : symbol × sort → sexpr atom
+| ⟨nm,s⟩ := sexpr.app nm [s]
+
+/-- Define a function in terms of inputs -/
+protected
+def define_fun {l} (nm:symbol) (args:list (symbol × sort)) {res:sort} (rhs : term l res) : cmd := do
+  ⟨sexpr.app (sexpr.of_string "define-fun" trivial) [ nm, sexpr.parens (args.map arg_pair), res, rhs ]⟩
+
+end cmd
+
+end smt2
