lean/deps/typed_smt2/src/galois/smt2/file_writer.lean
@@ -1,56 +1,18 @@
-import .interface
+import .cmd
 
 namespace smt2
 
-/-- An SMT command -/
-structure cmd :=
-(expr : sexpr)
-
-namespace cmd
-
-
-protected
-def write (c:cmd) (h:io.handle) : io punit := sexpr.write h (c.expr)
-
-protected
-def assert (p:term bool) : cmd := ⟨sexpr.app (by coerce "assert" sexpr)  [p.repr]⟩
-
-def symbol_is_sexpr : has_coe symbol sexpr := { coe := symbol.to_sexpr }
-
-local attribute [instance] symbol_is_sexpr
-
-/-- Declare a function -/
-protected
-def declare_fun (nm:symbol) (args:list sort) (res:sort) : cmd :=
-  ⟨sexpr.app (by coerce "declare-fun" sexpr) [nm, sexpr.of_list args, res]⟩
-
-/-- Declare a constant -/
-protected
-def declare_const (nm:symbol) (res:sort) : cmd :=
-  ⟨sexpr.app (by coerce "declare-const" sexpr) [nm, res]⟩
-
-/-- Map a symbol and sort pair from a function declaration to an s-expression -/
-def arg_pair : symbol × sort → sexpr
-| ⟨nm,s⟩ := sexpr.app nm [s]
-
-/-- Define a function in terms of inputs -/
-protected
-def define_fun (nm:symbol) (args:list (symbol × sort)) {res:sort} (rhs : term res) : cmd := do
-  ⟨sexpr.app (by coerce "define-fun" sexpr) [ nm, sexpr.of_list (args.map arg_pair), res, rhs.repr ]⟩
-
-end cmd
-
 /-- Interface for writing SMTLIB expressions to a handle or file. -/
-def file_writer := reader_t io.handle io
+def file_writer (l:logic) := reader_t io.handle io
 
 namespace file_writer
 
-instance : monad file_writer := by { unfold file_writer, apply_instance }
-instance : has_monad_lift io file_writer := by { unfold file_writer, apply_instance }
-instance : monad_reader io.handle file_writer := by { unfold file_writer, apply_instance }
+instance (l:logic) : monad (file_writer l) := by { unfold file_writer, apply_instance }
+instance (l:logic) : has_monad_lift io (file_writer l) := by { unfold file_writer, apply_instance }
+instance (l:logic) : monad_reader io.handle (file_writer l) := by { unfold file_writer, apply_instance }
 
 /-- Write a command to the file handle. -/
-def write (c:cmd) : file_writer punit := do
+def write {l:logic} (c:cmd) : file_writer l punit := do
   h ← read,
   monad_lift $ do
     c.write h,
@@ -58,44 +20,33 @@ def write (c:cmd) : file_writer punit := do
 
 /-- Assert a term is true. -/
 protected
-def assert (p:term bool) : file_writer punit := write (cmd.assert p)
+def assert {l:logic} (p:term l bool) : file_writer l punit := write (cmd.assert p)
 
 /-- Declare a function -/
-protected
-def declare_fun (nm:symbol) (args:list sort) (res:sort) : file_writer punit :=
+def declare_fun {l:logic} (nm:symbol) (args:list sort) (res:sort) : file_writer l punit :=
   write (cmd.declare_fun nm args res)
 
 /-- Declare a constant -/
-protected
-def declare_const (nm:symbol) (res:sort) : file_writer punit :=
+def declare_const {l:logic} (nm:symbol) (res:sort) : file_writer l punit :=
   write (cmd.declare_const nm res)
 
-/-- Map a symbol and sort pair from a function declaration to an s-expression -/
-def arg_pair : symbol × sort → sexpr
-| ⟨nm,s⟩ := sexpr.app nm.to_sexpr [s]
-
 /-- Define a function in terms of inputs -/
-protected
-def define_fun (nm:symbol) (args:list (symbol × sort)) {res:sort} (rhs : term res)
-: file_writer punit := do
+def define_fun {l:logic} (nm:symbol) (args:list (symbol × sort)) {res:sort} (rhs : term l res)
+: file_writer l punit := do
   write (cmd.define_fun nm args rhs)
 
-instance : is_generator file_writer :=
-{ assert        := file_writer.assert
-, declare_fun   := file_writer.declare_fun
-, declare_const := file_writer.declare_const
-, define_fun    := file_writer.define_fun
-}
+/-- Define a function in terms of inputs -/
+def check_sat{l:logic}  : file_writer l punit := do
+  write cmd.check_sat
 
 /-- Run the file writer -/
 protected
-def run {α} (path:string) (m:file_writer α) : io α := do
+def run {α} (l:logic) (path:string) (m:file_writer l α) : io α := do
   h ← io.mk_file_handle path io.mode.write tt,
   v ← m.run h,
   io.fs.close h,
   pure v
 
 end file_writer
-
 
 end smt2
