lean/deps/typed_smt2/src/galois/smt2/theories/bv.lean
@@ -1,0 +1,54 @@
+import data.bitvec
+
+import ..basic
+
+namespace smt2
+
+/-- SMTLIB bitvec sorts -/
+def bv (w : ℕ) : sort := ⟨symbol.of_string "BitVec" trivial, [w]⟩
+
+/-- Class for typings that interpret bitvectors correctly. -/
+class is_bv_logic (l:logic) :=
+(bv_correct : ∀(w:ℕ), l.type_of (bv w) = bitvec w)
+
+def logic.from_bitvec (l:logic) [is_bv_logic l] {w} (v:bitvec w) : l.type_of (bv w) :=
+  cast (eq.symm (is_bv_logic.bv_correct l w)) v
+
+def term.to_bitvec {l:logic} [is_bv_logic l] {w} (x:term l (bv w)) (m:model l) : bitvec w := cast (is_bv_logic.bv_correct l w) (x.interp m)
+
+namespace bv
+
+section
+parameters {l:logic}
+parameters [c:is_bv_logic l]
+include c
+
+/- Utility function to create a bitvector term assuming a compatible logic. -/
+def mk_term {w} (s:sexpr atom) (interp:model l → bitvec w) : term l (bv w) :=
+{ repr := s
+, interp := λm, l.from_bitvec (interp m)
+}
+
+/- Create a term from a decimal number -/
+def decimal {w:ℕ} (v:bitvec w) : term l (bv w) :=
+  mk_term ↑{ identifier
+           . head    := symbol.of_string "bv" trivial ++ symbol.of_nat v.to_nat
+           , indices := [w]
+           }
+          (λ_, v)
+
+
+/-- Bitvector addition -/
+def add {w:ℕ} (x y : term l (bv w)) : term l (bv w) :=
+  mk_term (sexpr.bin_app (symbol.of_string "bvadd" trivial) x y)
+          (λm, x.to_bitvec m + y.to_bitvec m)
+
+/-- Bitvector subtraction -/
+def sub {w:ℕ} (x y : term l (bv w)) : term l (bv w) :=
+  mk_term (sexpr.bin_app (symbol.of_string "bvsub" trivial) x y)
+          (λm, x.to_bitvec m + y.to_bitvec m)
+
+end
+end bv
+
+end smt2
